erasure/theories/ErasureUnquote.v
@@ -1,0 +1,41 @@
+(* Distributed under the terms of the MIT license. *)
+From Coq Require Import Program ssreflect ssrbool.
+From Equations Require Import Equations.
+Set Equations Transparent.
+From MetaCoq.Template Require Import config utils Kernames MCRelations Primitive.
+From MetaCoq.PCUIC Require Import PCUICAst PCUICAstUtils PCUICPrimitive.
+From MetaCoq.Erasure Require Import EAst EAstUtils EArities Extract Prelim EDeps ErasureProperties ErasureCorrectness.
+
+Set Asymmetric Patterns.
+Local Set Keyed Unification.
+Import MCMonadNotation.
+Implicit Types (cf : checker_flags).
+
+Definition unquote_prim_model {t : prim_tag} (e : @prim_model E.term t) : @prim_model PCUICAst.term t :=
+  match e in @prim_model _ x return prim_model _ x with
+  | primIntModel i => primIntModel i
+  | primFloatModel f => primFloatModel f
+  end.
+  
+Definition unquote_prim_val (p : prim_val E.term) : PCUICAst.prim_val :=
+  (p.π1; unquote_prim_model p.π2).
+
+#[bypass_check(guard)]  
+Fixpoint unquote (Σ : global_env) (t : term) (ty : PCUICAst.term) { struct t }: option PCUICAst.term :=
+  match t with
+  | tConstruct ind k args =>
+    let (hd, tyargs) := PCUICAstUtils.decompose_app ty in
+    match hd with
+    | PCUICAst.tInd ind' u' => 
+      '(mdecl, idecl, cdecl) <- PCUICAst.lookup_constructor Σ ind k ;;
+      unqargs <- monad_map2 (unquote Σ) tt 
+        (List.skipn mdecl.(PCUICEnvironment.ind_npars) args)
+        (map decl_type cdecl.(PCUICEnvironment.cstr_args)) ;;
+      let app := PCUICAst.mkApps (PCUICAst.tConstruct ind k u')
+        (List.firstn mdecl.(PCUICEnvironment.ind_npars) tyargs ++ unqargs)
+      in Some app
+    | _ => None
+    end
+  | tPrim pv => ret (PCUICAst.tPrim (unquote_prim_val pv))
+  | _ => None
+  end.
